

**Algebra (solving equations)**

To solve an equation for an unknown variable, we isolate the desired variable step-by-step. One of the easiest ways to do this is to undo the order of operations: for instance, addition and subtraction are the last to perform, so we undo addition with subtraction first.

**Example 1.**

$$\begin{aligned}
 4x + 1 &= 21 \\
 4x + 1 - 1 &= 21 - 1 \\
 4x &= 20 \\
 \frac{4x}{4} &= \frac{20}{4} \\
 x &= 5
 \end{aligned}$$

In practice, we typically skip the 2nd and 4th step, as it is clear what we did. The key idea when it comes to solving equations is that you **must perform the same operation to both sides of the equation**.

The distributive property says that

$$a(b + c) = ab + ac$$

for any real numbers  $a, b, c$ . This allows us to simplify certain equations in order to solve them. Note that unless otherwise specified, the preferred form of an answer is as a simplified, improper fraction.

**Example 2.**

$$\begin{aligned}
 2(x + 1) + 3(2x - 1) &= 9 \\
 2x + 2 + 6x - 3 &= 9 \\
 8x - 1 &= 9 \\
 8x &= 12 \\
 x &= \frac{12}{8} = \frac{3}{2}
 \end{aligned}$$

Be careful about negatives! I recommend grouping the sign with the coefficient so that you don't make a silly mistake. Remember that the product of two negatives is positive.

**Example 3.**

$$3x - 2(x - 1) = 3x + (-2)(x - 1) = 3x + (-2)(x) + (-2)(-1) = 3x - 2x + 2$$

NOT

$$3x - 2(x - 1) = 3x - 2(x) + 2(-1) = 3x - 2 - 1$$

When dealing with fractions, you have two main options: distribute as usual and solve with possibly fractional coefficients, or (my personal choice) clear the denominator by multiplying by the least common multiple of the denominators.

**Example 4.**

$$\frac{3x-1}{4} - \frac{6-x}{6} = \frac{2x-1}{3}$$

Method 1:

$$\begin{aligned}\frac{3x-1}{4} - \frac{6-x}{6} &= \frac{2x-1}{3} \\ \frac{3}{4}x - \frac{1}{4} - 1 + \frac{x}{6} &= \frac{2}{3}x - \frac{1}{3} \\ \left(\frac{3}{4} + \frac{1}{6} - \frac{2}{3}\right)x &= \frac{1}{4} + 1 - \frac{1}{3} \\ \frac{1}{4}x &= \frac{11}{12} \\ x &= \frac{11}{3}\end{aligned}$$

Method 2:

$$\begin{aligned}\frac{3x-1}{4} - \frac{6-x}{6} &= \frac{2x-1}{3} \\ 3(3x-1) - 2(6-x) &= 4(2x-1) \\ 9x-3-12+2x &= 8x-4 \\ 3x &= 11 \\ x &= \frac{11}{3}\end{aligned}$$

Notice it's easiest to simplify the fraction before moving on, so that

$$12 \cdot \frac{3x-1}{4} = 3(3x-1) \quad \text{NOT} \quad 12 \cdot \frac{3x-1}{4} = \frac{36x-12}{4}$$

Be careful not to multiply a single term more times than you are supposed to! A single term is composed of factors that are multiplied, so multiplying a term by a number means only one of the factors is multiplied (unless you break down the number into several smaller divisors).

$$2 \cdot \frac{3}{2} \left(\frac{1}{2}x - 1\right) = 3 \left(\frac{1}{2}x - 1\right) \quad \text{NOT} \quad 2 \cdot \frac{3}{2} \left(\frac{1}{2}x - 1\right) = 3(x-2)$$

1. Solve the following equations for  $x$ :

(a) (1 point)

$$4x + 7 = 23$$

(b) (1 point)

$$7x - 9 = 12$$

(c) (1 point)

$$5x + 8 = 2x + 20$$

2. Solve the following equations for  $x$ :

(a) (1 point)

$$3x - 5 = 16$$

(b) (1 point)

$$2x + 11 = 5x - 4$$

(c) (1 point)

$$6x + 9 = 3x + 18$$

3. Solve the following equations for  $x$ :

(a) (1 point)

$$8x - 7 = 3x + 18$$

(b) (1 point)

$$10 - 2x = 4x + 14$$

(c) (1 point)

$$7x + 5 = 2x + 20$$

4. Solve the following equations for  $x$ :

(a) (1 point)

$$3(2x + 4) - 5 = 19$$

(b) (1 point)

$$2(3x - 5) + 4(x + 1) = 18$$

(c) (1 point)

$$5(x + 2) - 3(2x - 1) = 7$$

5. Solve the following equations for  $x$ :

(a) (1 point)

$$4(2x - 3) + 3(1 - x) = 10$$

(b) (1 point)

$$2(5x + 1) - 4(x - 2) = 6$$

(c) (1 point)

$$3(x - 2) + 2(2x + 1) = 11$$

6. Solve the following equations for  $x$ :

(a) (1 point)

$$2(3x + 1) - 5(x - 2) = 4$$

(b) (1 point)

$$4(x - 3) - 2(2x + 1) = 6$$

(c) (1 point)

$$2(x + 3) - (x - 5) = x + 11$$



7. Solve the following equations for  $x$ :

(a) (1 point)

$$\frac{3x+2}{4} - \frac{x-1}{2} = 3$$

(b) (1 point)

$$\frac{2x-3}{5} + \frac{x+4}{3} = 7$$

8. Solve the following equations for  $x$ :

(a) (1 point)

$$\frac{3x-1}{4} + \frac{2x+3}{5} = \frac{7x+2}{6}$$

(b) (1 point)

$$\frac{5x+2}{3} - \frac{x-1}{2} = \frac{7x+5}{6}$$

9. Solve the following equations for  $x$ :

(a) (1 point)

$$\frac{2x+3}{5} + \frac{3x-4}{6} = \frac{5x+1}{4}$$

(b) (1 point)

$$\frac{4x-5}{7} - \frac{3x+2}{5} = \frac{2x-3}{3}$$

10. Solve the following equations for  $x$ :

(a) (1 point)

$$7(2x - 3) - 4(x + 5) = 3(2x + 1) + 8$$

(b) (1 point)

$$5(x - 2) - 3(2x + 1) + 4 = 2(3x - 4) - 1$$

11. Solve the following equations for  $x$ :

(a) (1 point)

$$\frac{3x+5}{4} + \frac{2x-3}{6} - \frac{x+1}{3} = \frac{5x-2}{12}$$

(b) (1 point)

$$\frac{5x-2}{3} - \frac{2x+1}{4} = \frac{3x-7}{6} + \frac{1}{2}$$

12. Solve the following equations for  $x$ :

(a) (1 point)

$$2(3x - 1) - \frac{4x + 5}{3} = 5x - 7 + \frac{x - 2}{2}$$

(b) (1 point)

$$\frac{3x - 2}{5} + 2(2x + 1) = \frac{7x + 4}{2} - \frac{x - 3}{10}$$

13. Solve the following equation for  $x$ :

$$\frac{2x+3}{4} - 3\left(\frac{x-1}{2} - 2\right) = \frac{5x-7}{6} + 2\left(\frac{x+2}{3} - 1\right)$$

14.

$$\frac{\frac{3x}{5} + 2}{\frac{1}{2}} - \frac{4 - \frac{x}{3}}{\frac{2}{3}} = \frac{\frac{5x}{6} - 1}{2} + \frac{3}{4}$$